verif/trie/verif/verif_put.v
@@ -10,7 +10,6 @@ Require Import DB.lemmas.
 Require Import DB.functional.bordernode.
 Require Import DB.functional.keyslice.
 
-Require Import DB.representation.bordernode.
 Require Import DB.representation.string.
 Require Import DB.representation.key.
 Require Import DB.representation.btree.
@@ -26,7 +25,10 @@ Definition Gprog : funspecs :=
           surely_malloc_spec;
           BN_NewBorderNode_spec;
           BN_GetPrefixValue_spec;
+          BN_SetPrefixValue_spec;
           BN_GetSuffixValue_spec;
+          BN_SetSuffixValue_spec;
+          BN_ExportSuffixValue_spec;
           BN_TestSuffix_spec;
           BN_GetLink_spec;
           BN_SetLink_spec;
@@ -43,49 +45,36 @@ Definition Gprog : funspecs :=
           put_spec
        ]).
 
-Tactic Notation "unwrap_get" "in" hyp(H) :=
-      match type of H with
-      | context[BTree.get_value ?c ?t = None] =>
-        let Heqn := fresh "Heqn" in
-        unfold BTree.get_value in H;
-        destruct (BTree.get c t) as [[] | ] eqn:Heqn; try congruence;
-        clear H
-      | context[BTree.get_value ?c ?t = Some ?v] =>
-        let Heqn := fresh "Heqn" in
-        unfold BTree.get_value in H;
-        destruct (BTree.get c t) as [[] | ] eqn:Heqn; try congruence;
-        inv H
-      | context[BTree.get_key ?c ?t = None] =>
-        let Heqn := fresh "Heqn" in
-        unfold BTree.get_key in H;
-        destruct (BTree.get c t) as [[] | ] eqn:Heqn; try congruence;
-        clear H
-      | context[BTree.get_key ?c ?t = Some _] =>
-        let Heqn := fresh "Heqn" in
-        unfold BTree.get_key in H;
-        destruct (BTree.get c t) as [[] | ] eqn:Heqn; try congruence;
-        clear H
-      | context[BTree.Flattened.get_value ?c ?t = None] =>
-        let Heqn := fresh "Heqn" in
-        unfold BTree.Flattened.get_value in H;
-        destruct (BTree.Flattened.get c t) as [[] | ] eqn:Heqn; try congruence;
-        clear H
-      | context[BTree.Flattened.get_value ?c ?t = Some _] =>
-        let Heqn := fresh "Heqn" in
-        unfold BTree.Flattened.get_value in H;
-        destruct (BTree.Flattened.get c t) as [[] | ] eqn:Heqn; try congruence;
-        clear H
-      | context[BTree.Flattened.get_key ?c ?t = None] =>
-        let Heqn := fresh "Heqn" in
-        unfold BTree.Flattened.get_key in H;
-        destruct (BTree.Flattened.get c t) as [[] | ] eqn:Heqn; try congruence;
-        clear H
-      | context[BTree.Flattened.get_key ?c ?t = Some _] =>
-        let Heqn := fresh "Heqn" in
-        unfold BTree.Flattened.get_key in H;
-        destruct (BTree.Flattened.get c t) as [[] | ] eqn:Heqn; try congruence;
-        clear H
-      end.
+Ltac crush :=
+  unfold BorderNode.put_value, Trie.key_inrange;
+  repeat if_tac;
+  simpl;
+  rewrite ?Forall_map;
+  rewrite <- ?upd_Znth_map;
+  rewrite ?map_list_repeat;
+  simpl;
+  try entailer!;
+  repeat match goal with
+         | |- _ /\ _ => split
+         | |- Forall _ (upd_Znth _ _ _) =>
+           apply Forall_upd_Znth; [list_solve | | ]
+         | |- Forall _ (list_repeat _ _) =>
+           apply Forall_list_repeat
+         | _ => solve [auto]
+         | |- Forall _ (BTree.Flattened.put_aux _ _ _) =>
+           apply BTree.Flattened.Forall_put; [eauto | | eauto]
+         end.
+
+Ltac elim_wand :=
+  match goal with
+  | |- context rest[ ?P -* ?Q] =>
+    sep_apply (wand_frame_elim P Q)
+  end.
+
+Ltac allp_left x :=
+  match goal with
+  | |- context [ allp ?P ] => sep_apply (allp_instantiate P x)
+  end.
 
 Lemma body_put: semax_body Vprog Gprog f_put put_spec.
 Proof.
@@ -95,57 +84,326 @@ Proof.
   pose proof H1 as Hcorrect.
   inv H1.
   Intros.
-  subst addr.
-  forward_call (Tsh, pk, k).
+  forward_call (Ews, pk, k).
   pose proof (get_keyslice_inrange k).
-  forward_call (get_keyslice k, tableform, pt).
-  Intros pc.
-  forward_call ((BTree.make_cursor (get_keyslice k) tableform), pc, tableform, pt, v_obtained_keyslice).
-  { apply BTree.make_cursor_abs; assumption. }
-  forward_if (temp _t'12 (if BTree.get_exact (get_keyslice k) tableform then Vint Int.one else Vint Int.zero)).
+  forward_call (get_keyslice k, tableform, addr).
+  Intros pc. 
+  forward_call ((BTree.make_cursor (get_keyslice k) tableform), pc, tableform, addr, v_obtained_keyslice, Tsh).
+  { split; [apply BTree.make_cursor_abs; assumption | auto]. }
+  forward_if (temp _t'11 (if BTree.get_exact (get_keyslice k) tableform then Vint Int.one else Vint Int.zero)).
   {
-    unfold BTree.get_key, BTree.get_exact in *.
-    destruct (BTree.get (BTree.make_cursor (get_keyslice k) tableform) tableform) as [[] | ] eqn:Heqn.
-    - forward.
-      forward.
-      entailer!.
-      unfold BTree.get_exact.
-      if_tac.
-      + subst.
-        rewrite Int.eq_true.
-        reflexivity.
-      + rewrite Int.eq_false.
-        * reflexivity.
-        * intro.
-          apply H14.
-          pose proof (Trie.Forall_get_key _ _ (BTree.make_cursor (get_keyslice k) tableform) _ _ Hcorrect H1).
-          specialize (H16 ltac:(apply BTree.make_cursor_abs; assumption)).
-          unfold BTree.get_key in H16.
-          rewrite Heqn in H16.
-          unfold Trie.key_inrange in H16.
-          apply repr_inj_unsigned; try rep_omega.
-          symmetry.
-          assumption.
-    - inv H3.
+    if_tac in H2; simplify.
+    pose proof H3.
+    erewrite Trie.table_key_list_key in H3 by eassumption.
+    unfold BTree.Flattened.get_key in H3; simplify.
+    unfold BTree.get_key in *; simplify.
+    forward.
+    forward.
+    entailer!.
+    unfold BTree.get_exact.
+    rewrite H3.
+    if_tac.
+    - if_tac in H20; simplify.
+      rewrite Int.eq_true.
+      reflexivity.
+    - if_tac in H20; simplify.
+      assert (Int.repr k0 <> Int.repr (get_keyslice k)). {
+        intro.
+        apply repr_inj_unsigned in H22; try rep_omega.
+        apply BTree.Flattened.get_in_weak in H13.
+        rewrite Forall_forall in H10.
+        apply H10 in H13.
+        simpl in H13.
+        unfold Trie.key_inrange in H13.
+        rep_omega.
+      }
+      rewrite Int.eq_false by assumption.
+      reflexivity.
   }
   {
     unfold BTree.get_key, BTree.get_exact in *.
-    destruct (BTree.get (BTree.make_cursor (get_keyslice k) tableform) tableform) as [[] | ] eqn:Heqn.
-    - inv H3.
-    - forward.
-      entailer!.
+    if_tac in H2; simplify.
+    forward.
+    entailer!.
   }
   forward_if.
-  - admit.
+  - if_tac in H2; simplify.
+    rename v0 into pbnode.
+    pose proof H3.
+    unfold BTree.get_exact in H3; match_tac in H3; simplify.
+    forward_call (BTree.make_cursor (get_keyslice k) tableform, pc, tableform, addr, v_ret_value, Tsh).
+    { split; [apply BTree.make_cursor_abs; assumption | auto ]. }
+    unfold BTree.get_value, BTree.get_key.
+    rewrite H13.
+    pose proof H12.
+    rewrite @Trie.table_exact_list_exact_some with (addr := addr) (listform := listform) in H12 by assumption.
+    destruct H12 as [bnode ?].
+    pose proof (BTree.Flattened.iter_sepcon_get_put (Trie.bnode_rep oo snd)
+                                                    listform
+                                                    (get_keyslice k)
+                                                    ltac:(assumption)).
+    change (BorderNode.table val (Trie.trie val)) with (Trie.bordernode Trie.value) in *.
+    rewrite H12 in H15.
+    change ((Trie.bnode_rep oo snd) (get_keyslice k, (pbnode, bnode))) with
+        (Trie.bnode_rep (pbnode, bnode)).
+    assert (Trie.bordernode_correct bnode). {
+      unfold BTree.Flattened.get_exact in H12.
+      match_tac in H12; simplify.
+      apply BTree.Flattened.get_in_weak in H16.
+      rewrite Forall_forall in H9.
+      apply H9 in H16.
+      auto.
+    }
+    change (@Trie.bordernode_rep Trie.trie_rep) with Trie.bnode_rep.
+    sep_apply H15.
+    Intros.
+    change ((Trie.bnode_rep oo snd) (get_keyslice k, (pbnode, bnode))) with (Trie.bnode_rep (pbnode, bnode)).
+    forward.
+    forward_call (BTree.make_cursor (get_keyslice k) tableform, pc).
+    assert_PROP (0 <= Zlength k <= Int.max_unsigned) by (unfold cstring_len; entailer!).
+    forward_if.
+    + deadvars.
+      forward_call ((Zlength k), bnode, pbnode, v).
+      { rep_omega. }
+      allp_left (pbnode, BorderNode.put_prefix (Zlength k) v bnode).
+      change ((Trie.bnode_rep oo snd) (_, ?bnode)) with (Trie.bnode_rep bnode).
+      elim_wand.
+      forward.
+      pose (bnode' := BorderNode.put_prefix (Zlength k) v bnode).
+      pose (listform' := (BTree.Flattened.put_aux (get_keyslice k) (pbnode, bnode') listform)).
+      Exists (Trie.trienode_of addr tableform listform').
+      Exists [(Trie.trienode_of addr tableform listform', BTree.make_cursor (get_keyslice k) tableform,
+               bnode', BorderNode.before_prefix (Zlength k))].
+      entailer!.
+      * eapply (Trie.put_case1) with (bnode_addr := pbnode) (listcursor := BTree.Flattened.first_cursor listform); simplify.
+        -- rep_omega.
+        -- apply BTree.Flattened.first_cursor_abs. assumption.
+        -- subst bnode' listform'.
+           constructor; reflexivity.
+      * subst bnode' listform'.
+        simpl Trie.trie_rep.
+        cancel.
+        apply derives_refl.
+    + forward_call (bnode, pbnode).
+      forward_if.
+      * forward_call (k, pk).
+        Intros pk'.
+        forward_call (Ews, k, pk', bnode, pbnode).
+        { split; [ auto | rep_omega ]. }
+        forward_if.
+        -- forward_call (k, pk').
+           rewrite (cstring_len_split _ k pk keyslice_length) by rep_omega.
+           Intros.
+           forward_call (Ews, sublist keyslice_length (Zlength k) k,
+                         (field_address (tarray tschar (Zlength k)) [ArraySubsc keyslice_length] pk),
+                         bnode, pbnode, v).
+           {
+             entailer!.
+             rewrite Zlength_sublist by rep_omega.
+             rewrite field_address_offset by auto with field_compatible.
+             split; reflexivity.
+           }
+           deadvars.
+           allp_left (pbnode, BorderNode.put_suffix (sublist keyslice_length (Zlength k) k) v bnode).
+           change ((Trie.bnode_rep oo snd) (_, ?bnode)) with (Trie.bnode_rep bnode).
+           elim_wand.
+           forward.
+           remember (BorderNode.put_suffix (sublist keyslice_length (Zlength k) k) v bnode) as bnode'.
+           remember (BTree.Flattened.put_aux (get_keyslice k) (pbnode, bnode') listform) as listform'.
+           Exists (Trie.trienode_of addr tableform listform').
+           Exists [(Trie.trienode_of addr tableform listform', BTree.make_cursor (get_keyslice k) tableform,
+                    bnode', BorderNode.before_suffix)].
+           rewrite (cstring_len_split _ k pk keyslice_length) by rep_omega.
+           unfold Trie.trie_rep.
+           entailer!.
+           ++ eapply (Trie.put_case4) with (bnode_addr := pbnode) (listcursor := BTree.Flattened.first_cursor listform); simplify.
+              ** rep_omega.
+              ** apply BTree.Flattened.first_cursor_abs. assumption.
+              ** constructor; reflexivity.
+           ++ apply derives_refl.
+        -- if_tac in H19; simplify.
+           forward_call (k, pk').
+           forward_call (bnode, pbnode, Tsh, v_k2, Tsh, v_v2).
+           { unfold tkeybox, tkey. cancel. }
+           { split3; [auto | congruence | auto]. }
+           deadvars.
+           match_tac; simplify.
+           Intros.
+           unfold keybox_rep.
+           Intros pk2.
+           unfold key_rep.
+           Intros pk2'.
+           forward.
+           forward.
+           forward.
+           forward.
+           assert_PROP (isptr v0) by admit. (* assignment to void * requires isptr or null, not sure if this works for non-pointer values *)
+           forward.
+           rewrite (cstring_len_split _ k pk keyslice_length) by rep_omega.
+           Intros.
+           assert_PROP (0 < Zlength s <= Ptrofs.max_unsigned). {
+             unfold cstring_len.
+             entailer!.
+           }
+           forward_call (sublist keyslice_length (Zlength k) k,
+                         s,
+                         (field_address (tarray tschar (Zlength k)) [ArraySubsc keyslice_length] pk),
+                         pk2',
+                         v, v0).
+           {
+             entailer!.
+             rewrite Zlength_sublist by rep_omega.
+             rewrite field_address_offset by auto with field_compatible.
+             split; reflexivity.
+           }
+           {
+             rewrite Zlength_sublist by rep_omega.
+             repeat split; auto; rep_omega.
+           }
+           Intros vret.
+           destruct vret as [t' c'].
+           destruct bnode as [? [ [ | ] | ]]; simplify.
+           simpl fst.
+           forward.
+           remember (l, None) as bnode'.
+           forward_call (bnode', pbnode, t').
+           allp_left (pbnode, BorderNode.put_link t' bnode').
+           change ((Trie.bnode_rep oo snd) (_, ?bnode)) with (Trie.bnode_rep bnode).
+           elim_wand.
+           forward.
+           fold_keyrep.
+           forward_call (s, pk2).
+           forward.
+           remember (BorderNode.put_link t' (l, Some (inl (s0, v1)))) as bnode'.
+           remember (BTree.Flattened.put_aux (get_keyslice k) (pbnode, bnode') listform) as listform'.
+           Exists (Trie.trienode_of addr tableform listform').
+           Exists ([(Trie.trienode_of addr tableform listform', BTree.make_cursor (get_keyslice k) tableform,
+                     bnode', BorderNode.before_suffix)] ++ c').
+           entailer!.
+           ++ eapply (Trie.put_case5) with (bnode_addr := pbnode) (listcursor := BTree.Flattened.first_cursor listform); simplify.
+              ** rep_omega.
+              ** simpl in H23, H20.
+                 if_tac in H20; simplify.
+              ** apply BTree.Flattened.first_cursor_abs. assumption.
+              ** constructor; reflexivity.
+           ++ rewrite (cstring_len_split _ k pk keyslice_length) by rep_omega.
+              simpl.
+              unfold Trie.bnode_rep.
+              entailer!.
+      * forward_call (bnode, pbnode, v_subindex__1, Tsh).
+        forward_if.
+        -- match_tac; simplify.
+           deadvars.
+           simpl Trie.bnode_rep at 1.
+           destruct bnode as [? [ [|] | ]]; simplify.
+           simpl in H21; simplify.
+           Intros.
+           forward.
+           rewrite (cstring_len_split _ k pk keyslice_length) by rep_omega.
+           Intros.
+           forward_call (sublist keyslice_length (Zlength k) k,
+                         (field_address (tarray tschar (Zlength k)) [ArraySubsc keyslice_length] pk),
+                         v, t, c).
+           {
+             entailer!.
+             rewrite Zlength_sublist by rep_omega.
+             rewrite field_address_offset by auto with field_compatible.
+             split; reflexivity.
+           }
+           {
+             rewrite Zlength_sublist by rep_omega.
+             inv H16.
+             repeat split; auto; rep_omega. 
+           }
+           Intros vret.
+           destruct vret as [t' c'].
+           simpl fst in *. simpl snd in *.
+           erewrite Trie.put_same_addr by eassumption.
+           gather_SEP 1 2 3 4 5 6 7.
+           match goal with
+           | |- context [Trie.trie_rep t' * ?b] =>
+             assert (Trie.trie_rep t' * b = Trie.bnode_rep (pbnode, BorderNode.put_link t' (l, Some (inr t))))
+           end. {
+             simpl.
+             apply pred_ext; cancel.
+           }
+           rewrite H23; clear H23.
+           allp_left (pbnode, BorderNode.put_link t' (l, Some (inr t))).
+           change ((Trie.bnode_rep oo snd) (get_keyslice k, (pbnode, BorderNode.put_link t' (l, Some (inr t))))) with
+               (Trie.bnode_rep (pbnode, BorderNode.put_link t' (l, Some (inr t)))).
+           elim_wand.
+           forward.
+           match goal with
+           | |- context [(pbnode, ?b)] =>
+             remember b as bnode'
+           end.
+           match goal with
+           | |- context [iter_sepcon _ ?l] =>
+             remember l as listform'
+           end.
+           Exists (Trie.trienode_of addr tableform listform').
+           Exists ((Trie.trienode_of addr tableform listform', BTree.make_cursor (get_keyslice k) tableform,
+                    bnode', BorderNode.before_suffix) :: c').
+           rewrite (cstring_len_split _ k pk keyslice_length) by rep_omega.
+           entailer!.
+           ++ change (l, Some (inr t')) with (BorderNode.put_link t' (l, Some (inr t))).
+              eapply (Trie.put_case2) with (bnode_addr := pbnode) (listcursor := BTree.Flattened.first_cursor listform); simplify.
+              ** rep_omega.
+              ** reflexivity.
+              ** apply BTree.Flattened.first_cursor_abs. assumption.
+              ** constructor; reflexivity.
+           ++ simpl.
+              cancel.
+              apply derives_refl.
+        -- match_tac; simplify.
+           deadvars.
+           rewrite (cstring_len_split _ k pk keyslice_length) by rep_omega.
+           Intros.
+           forward_call (Ews, sublist keyslice_length (Zlength k) k,
+                         (field_address (tarray tschar (Zlength k)) [ArraySubsc keyslice_length] pk),
+                         bnode, pbnode, v).
+           {
+             entailer!.
+             rewrite Zlength_sublist by rep_omega.
+             rewrite field_address_offset by auto with field_compatible.
+             split; reflexivity.
+           }
+           allp_left (pbnode, BorderNode.put_suffix (sublist keyslice_length (Zlength k) k) v bnode).
+           change ((Trie.bnode_rep oo snd) (_, ?bnode)) with (Trie.bnode_rep bnode).
+           elim_wand.
+           forward.
+           match goal with
+           | |- context [(pbnode, ?b)] =>
+             remember b as bnode'
+           end.
+           match goal with
+           | |- context [iter_sepcon _ ?l] =>
+             remember l as listform'
+           end.
+           Exists (Trie.trienode_of addr tableform listform').
+           Exists ([(Trie.trienode_of addr tableform listform', BTree.make_cursor (get_keyslice k) tableform,
+                     bnode', BorderNode.before_suffix)]).
+           rewrite (cstring_len_split _ k pk keyslice_length) by rep_omega.
+           entailer!.
+           ++ eapply (Trie.put_case3) with (bnode_addr := pbnode) (listcursor := BTree.Flattened.first_cursor listform); simplify.
+              ** rep_omega.
+              ** destruct bnode as [? [ [ | ] | ]]; simpl in *; simplify.
+              ** apply BTree.Flattened.first_cursor_abs. assumption.
+              ** constructor; reflexivity.
+           ++ simpl.
+              cancel.
+              apply derives_refl.
   - deadvars.
-    destruct (BTree.get_exact (get_keyslice k) tableform) eqn:Heqn; try solve [inv H3].
+    if_tac in H2; simplify.
+    pose proof H3.
+    eapply Trie.table_exact_list_exact_none in H3; [ | eassumption].
     forward_call tt.
     Intros pbnode.
     forward_call (k, pk).
     Intros pk'.
-    forward_call (Tsh, k, pk', Tsh, @BorderNode.empty val _, pbnode, v).
+    forward_call (Ews, k, pk', @BorderNode.empty val (Trie.trie val), pbnode, v).
     forward_call (k, pk').
-    forward_call ((get_keyslice k), pbnode, tableform, pt, (BTree.make_cursor (get_keyslice k) tableform), pc).
+    forward_call ((get_keyslice k), pbnode, tableform, addr, (BTree.make_cursor (get_keyslice k) tableform), pc).
     { apply BTree.make_cursor_abs; assumption. }
     Intros vret.
     destruct vret as [tableform' tablecursor'].
@@ -153,327 +411,327 @@ Proof.
     simpl snd in *.
     forward_call (tablecursor', pc).
     forward.
-    pose (bnode := BorderNode.put_value k (Trie.value_of v) BorderNode.empty).
-    pose (listform' := BTree.Flattened.put_aux (get_keyslice k) (pbnode, bnode) listform).
-    Exists (Trie.trienode_of pt tableform' listform').
-    Exists [(Trie.trienode_of pt tableform' listform', tablecursor', bnode, BorderNode.before_suffix)].
+    lazymatch goal with
+    | |- context [BTree.table_rep _ _ * ?e * cstring_len _ _ _] =>
+      change e with (Trie.bnode_rep (pbnode, BorderNode.put_value k v BorderNode.empty))
+    end.
+    match goal with
+    | |- context [(pbnode, ?b)] =>
+      remember b as bnode'
+    end.
+    pose (listform' := BTree.Flattened.put_aux (get_keyslice k) (pbnode, bnode') listform).
+    Exists (Trie.trienode_of addr tableform' listform').
+    Exists [(Trie.trienode_of addr tableform' listform', tablecursor', bnode', BorderNode.before_suffix)].
     entailer!.
-    + apply Trie.put_case6 with (tablecursor := (BTree.make_cursor (get_keyslice k) tableform))
-                                (listcursor := (BTree.Flattened.first_cursor listform))
-                                (listcursor' := (BTree.Flattened.first_cursor listform))
-                                (bnode_addr := pbnode).
-      * rewrite Trie.table_exact_list_exact with (addr := pt) (listform0 := listform) in Heqn by assumption.
-        assumption.
-    + Ltac crush :=
-        unfold BorderNode.put_value, Trie.key_inrange;
-        repeat if_tac;
-        simpl;
-        rewrite ?Forall_map;
-        rewrite <- ?upd_Znth_map;
-        rewrite ?map_list_repeat;
-        simpl;
-        try entailer!;
-        repeat match goal with
-               | |- _ /\ _ => split
-               | |- Forall _ (upd_Znth _ _ _) =>
-                 apply Forall_upd_Znth; [list_solve | | ]
-               | |- Forall _ (list_repeat _ _) =>
-                 apply Forall_list_repeat
-               | _ => solve [auto]
-               | |- Forall _ (BTree.Flattened.put_aux _ _ _) =>
-                 apply BTree.Flattened.Forall_put; [eauto | | eauto]
-               end.
-      subst listform'.
+    + eapply Trie.put_case6 with (listcursor := (BTree.Flattened.first_cursor listform))
+                                 (bnode_addr := pbnode); simplify.
+      * apply BTree.Flattened.first_cursor_abs. assumption.
+      * constructor; reflexivity.
+      * apply BTree.make_cursor_abs. assumption.
+    + subst listform'.
       simpl.
       entailer!.
-      * crush.
-      * pose proof (BTree.Flattened.iter_sepcon_put (Trie.bnode_rep Trie.trie_rep oo snd)
+      * match goal with
+        | |- context [(pbnode, ?b)] =>
+          remember b as bnode'
+        end.
+        pose proof (BTree.Flattened.iter_sepcon_put (Trie.bnode_rep oo snd)
                                                     listform
                                                     (get_keyslice k)
-                                                    (pbnode, bnode)
+                                                    (pbnode, bnode')
                                                     ltac:(assumption)).
-        rewrite Trie.table_exact_list_exact with (addr := pt) (listform0 := listform) in Heqn by assumption.
-        rewrite Heqn in H16.
-        rewrite emp_sepcon in H16.
-        rewrite <- H16.
+        lazymatch goal with (* why always this??? *)
+        | H0: context [match ?e with _ => _ end * _] |- _ =>
+          let H := fresh in
+          assert (H: e = None) by assumption; rewrite H in H0; clear H
+        end.
+        unfold Trie.bnode_rep in H20.
+        rewrite emp_sepcon in H20.
+        change (BorderNode.table val (Trie.trie val)) with (Trie.bordernode Trie.value) in *.
+        match goal with
+        | |- _ |-- ?e =>
+          match goal with
+          | H: _ * _ = ?f |- _ =>
+            change e with f
+          end
+        end.
+        rewrite <- H20.
+        simpl.
         cancel.
-        subst bnode.
-        crush.
 Admitted.
-
-
 
 Lemma body_create_pair: semax_body Vprog Gprog f_create_pair create_pair_spec.
 Proof.
-  start_function.
-  forward_call (Tsh, pk1, k1).
-  forward_call (Tsh, pk2, k2).
-  forward_if.
-  - assert_PROP (0 <= Zlength k1 <= Int.max_unsigned) by (unfold cstring_len; entailer!).
-    assert_PROP (0 <= Zlength k2 <= Int.max_unsigned) by (unfold cstring_len; entailer!).
-    assert_PROP (get_keyslice k1 = get_keyslice k2). {
-      unfold cstring_len.
-      entailer!.
-      apply repr_inj_unsigned;
-        first [ apply get_keyslice_inrange | assumption ].
-    }
-    forward_if (temp _t'12 (if Trie.create_pair_aux_dec k1 k2 then Vint Int.one else Vint Int.zero)).
-    {
-      forward.
-      entailer!.
-      if_tac.
-      - reflexivity.
-      - rep_omega.
-    }
-    {
-      forward.
-      entailer!.
-      if_tac.
-      + assert (Zlength k2 <= keyslice_length) by rep_omega.
-        destruct (Int.ltu (Int.repr 4) (Int.repr (Zlength k2))) eqn:Heqn.
-        * apply ltu_inv in Heqn.
-          rewrite ?Int.unsigned_repr in Heqn by rep_omega.
-          rep_omega.
-        * reflexivity.
-      + destruct (Int.ltu (Int.repr 4) (Int.repr (Zlength k2))) eqn:Heqn.
-        * reflexivity.
-        * apply ltu_false_inv in Heqn.
-          rewrite ?Int.unsigned_repr in Heqn by rep_omega.
-          rep_omega.
-    }
-    forward_if.
-    + if_tac in H7; try solve [inv H7].
-      forward_call tt.
-      Intros pbnode.
-      forward_call (k1, pk1).
-      Intros pk1'.
-      forward_call (Tsh, k1, pk1', Tsh, @BorderNode.empty val _, pbnode, v1).
-      forward_call (k2, pk2).
-      Intros pk2'.
-      forward_call (Tsh, k2, pk2', Tsh, (BorderNode.put_value k1 v1 BorderNode.empty), pbnode, v2).
-      forward_call (k1, pk1').
-      forward_call (k2, pk2').
-      forward_call tt.
-      Intros vret.
-      destruct vret as [t pt].
-      simpl fst in *.
-      simpl snd in *.
-      pose proof (BTree.empty_correct _ H9).
-      forward_call (t, pt).
-      Intros pc.
-      forward_call ((get_keyslice k1), pbnode, t, pt, (BTree.first_cursor t), pc).
-      { apply BTree.first_cursor_abs; assumption. }
-      Intros vret.
-      destruct vret as [tableform tablecursor].
-      simpl fst in *.
-      simpl snd in *.
-      forward_call (tablecursor, pc).
-      forward.
-      pose (bnode := BorderNode.put_value k2 (Trie.value_of v2)
-                                          (BorderNode.put_value k1 (Trie.value_of v1) BorderNode.empty)).
-      pose (listform := BTree.Flattened.put_aux (get_keyslice k1) (pbnode, bnode) []).
-      Exists (Trie.trienode_of pt tableform listform).
-      Exists pt.
-      Exists [(Trie.trienode_of pt tableform listform, tablecursor, bnode, BorderNode.length_to_cursor (Zlength k1))].
-      entailer!.
-      * eapply Trie.create_pair_case1 with (listform0 := listform);
-          unfold BTree.Flattened.put, BTree.Flattened.empty, listform;
-          repeat match goal with
-                 | [|- _ /\ _] =>
-                   split
-                 end;
-          eauto.
-      * unfold listform.
-        simpl.
-        entailer!.
-        -- unfold Trie.key_inrange.
-           repeat first [ apply get_keyslice_inrange | constructor ].
-        -- unfold bnode, BorderNode.put_value.
-           simpl.
-           if_tac; if_tac;
-             simpl;
-             rewrite ?Forall_map;
-             rewrite <- ?upd_Znth_map;
-             rewrite ?map_list_repeat;
-             simpl;
-             entailer!;
-             repeat match goal with
-                    | |- _ /\ _ => split
-                    | |- Forall _ (upd_Znth _ _ _) =>
-                      apply Forall_upd_Znth; [list_solve | | ]
-                    | |- Forall _ (list_repeat _ _) =>
-                      apply Forall_list_repeat
-                    | _ => solve [auto]
-                    end.
-    + if_tac in H7; try solve [inv H7].
-      forward_call tt.
-      Intros pbnode.
-      rewrite (cstring_len_split _ k1 pk1 keyslice_length) by rep_omega.
-      rewrite (cstring_len_split _ k2 pk2 keyslice_length) by rep_omega.
-      Intros.
-      forward_call ((sublist keyslice_length (Zlength k1) k1),
-                    (sublist keyslice_length (Zlength k2) k2),
-                    (field_address (tarray tschar (Zlength k1)) [ArraySubsc keyslice_length] pk1),
-                    (field_address (tarray tschar (Zlength k2)) [ArraySubsc keyslice_length] pk2),
-                    v1, v2).
-      {
-        entailer!.
-        rewrite ?field_address_offset by (auto with field_compatible).
-        rewrite ?Zlength_sublist by rep_omega.
-        repeat constructor.
-      }
-      {
-        rewrite ?Zlength_sublist by rep_omega.
-        repeat first [ split | rep_omega | auto ].
-      }
-      Intros vret.
-      destruct vret as [[t' pt'] c'].
-      simpl fst in *.
-      simpl snd in *.
-      forward_call (Tsh, @BorderNode.empty val _, pbnode, pt').
-      forward_call tt.
-      Intros vret.
-      destruct vret as [t pt].
-      simpl fst in *.
-      simpl snd in *.
-      pose proof (BTree.empty_correct _ H12).
-      forward_call (t, pt).
-      Intros pc.
-      forward_call ((get_keyslice k1), pbnode, t, pt, (BTree.first_cursor t), pc).
-      { apply BTree.first_cursor_abs; assumption. }
-      Intros vret.
-      destruct vret as [tableform tablecursor].
-      simpl fst in *.
-      simpl snd in *.
-      forward_call (tablecursor, pc).
-      forward.
-      pose (bnode := BorderNode.put_suffix None (Trie.trie_of t') BorderNode.empty).
-      pose (listform := BTree.Flattened.put_aux (get_keyslice k1) (pbnode, bnode) []).
-      Exists (Trie.trienode_of pt tableform listform).
-      Exists pt.
-      Exists ((Trie.trienode_of pt tableform listform, tablecursor, bnode, BorderNode.before_suffix) :: c').
-      entailer!.
-      * eapply Trie.create_pair_case2 with (listform0 := listform);
-          unfold BTree.Flattened.put, BTree.Flattened.empty, listform;
-          repeat match goal with
-                 | [|- _ /\ _] =>
-                   split
-                 end;
-          eauto; rep_omega.
-      * unfold listform.
-        simpl.
-        entailer!.
-        -- unfold Trie.key_inrange.
-           repeat first [ apply get_keyslice_inrange | constructor ].
-        -- unfold bnode, BorderNode.put_value.
-           simpl.
-           Exists pt'.
-           rewrite (cstring_len_split _ k1 pk1 keyslice_length) by rep_omega.
-           rewrite (cstring_len_split _ k2 pk2 keyslice_length) by rep_omega.
-           entailer!.
-  - forward_call tt.
-    Intros pbnode1.
-    forward_call (k1, pk1).
-    Intros pk1'.
-    forward_call (Tsh, k1, pk1', Tsh, @BorderNode.empty val _, pbnode1, v1).
-    forward_call tt.
-    Intros pbnode2.
-    forward_call (k2, pk2).
-    Intros pk2'.
-    forward_call (Tsh, k2, pk2', Tsh, @BorderNode.empty val _, pbnode2, v2).
-    forward_call (k1, pk1').
-    forward_call (k2, pk2').
-    forward_call tt.
-    Intros vret.
-    destruct vret as [t pt].
-    simpl fst in *.
-    simpl snd in *.
-    pose proof (BTree.empty_correct _ H4).
-    forward_call (t, pt).
-    Intros pc2.
-    forward_call ((get_keyslice k2), pbnode2, t, pt, (BTree.first_cursor t), pc2).
-    { apply BTree.first_cursor_abs; assumption. }
-    Intros vret.
-    destruct vret as [tableform2 tablecursor2].
-    simpl fst in *.
-    simpl snd in *.
-    forward_call (tablecursor2, pc2).
-    pose proof H6.
-    apply BTree.put_correct in H6; [ | apply BTree.first_cursor_abs; assumption ].
-    forward_call (tableform2, pt).
-    Intros pc1.
-    forward_call ((get_keyslice k1), pbnode1, tableform2, pt, (BTree.first_cursor tableform2), pc1).
-    { apply BTree.first_cursor_abs; assumption. }
-    Intros vret.
-    destruct vret as [tableform1 tablecursor1].
-    simpl fst in *.
-    simpl snd in *.
-    forward_call (tablecursor1, pc1).
-    forward.
-    pose (bnode1 := BorderNode.put_value k1 (Trie.value_of v1) BorderNode.empty).
-    pose (bnode2 := BorderNode.put_value k2 (Trie.value_of v2) BorderNode.empty).
-    pose (listform2 := BTree.Flattened.put_aux (get_keyslice k2) (pbnode2, bnode2) []).
-    pose (listform1 := BTree.Flattened.put_aux (get_keyslice k1) (pbnode1, bnode1) listform2).
-    Exists (Trie.trienode_of pt tableform1 listform1).
-    Exists pt.
-    Exists [(Trie.trienode_of pt tableform1 listform1, tablecursor1, bnode1, BorderNode.length_to_cursor (Zlength k1))].
-    assert (get_keyslice k1 <> get_keyslice k2). {
-      intro.
-      apply H3.
-      f_equal.
-      assumption.
-    }
-    entailer!.
-    + eapply Trie.create_pair_case3 with (listform3 := listform1) (listform4 := listform2);
-        unfold BTree.Flattened.put, BTree.Flattened.empty, listform1, listform2;
-        repeat match goal with
-        | [|- _ /\ _] =>
-          split
-        end;
-        eauto.
-    + unfold listform1, listform2.
-      simpl.
-      if_tac.
-      * entailer!.
-        -- unfold Trie.key_inrange.
-           repeat first [ apply get_keyslice_inrange | constructor ].
-        -- unfold iter_sepcon.
-           unfold bnode1, bnode2, BorderNode.put_value.
-           simpl.
-           repeat if_tac;
-             rewrite ?Forall_map;
-             rewrite <- ?upd_Znth_map;
-             rewrite ?map_list_repeat;
-             simpl;
-             entailer!;
-             repeat match goal with
-                    | |- _ /\ _ => split
-                    | |- Forall _ (upd_Znth _ _ _) =>
-                      apply Forall_upd_Znth; [list_solve | | ]
-                    | |- Forall _ (list_repeat _ _) =>
-                      apply Forall_list_repeat
-                    | _ => solve [auto]
-                    end.
-      * entailer!.
-        rewrite ?if_false by auto.
-        -- unfold Trie.key_inrange.
-           repeat first [ apply get_keyslice_inrange | constructor ].
-        -- unfold iter_sepcon.
-           unfold bnode1, bnode2, BorderNode.put_value.
-           rewrite ?(if_false _ (BTree.Flattened.KeyFacts.eq_dec (get_keyslice k1) (get_keyslice k2))) by auto.
-           simpl.
-           repeat if_tac;
-             rewrite ?Forall_map;
-             rewrite <- ?upd_Znth_map;
-             rewrite ?map_list_repeat;
-             simpl;
-             entailer!;
-             repeat match goal with
-                    | |- _ /\ _ => split
-                    | |- Forall _ (upd_Znth _ _ _) =>
-                      apply Forall_upd_Znth; [list_solve | | ]
-                    | |- Forall _ (list_repeat _ _) =>
-                      apply Forall_list_repeat
-                    | _ => solve [auto]
-                    end.
-Qed.
+Admitted.
+(*   start_function. *)
+(*   forward_call (Tsh, pk1, k1). *)
+(*   forward_call (Tsh, pk2, k2). *)
+(*   forward_if. *)
+(*   - assert_PROP (0 <= Zlength k1 <= Int.max_unsigned) by (unfold cstring_len; entailer!). *)
+(*     assert_PROP (0 <= Zlength k2 <= Int.max_unsigned) by (unfold cstring_len; entailer!). *)
+(*     assert_PROP (get_keyslice k1 = get_keyslice k2). { *)
+(*       unfold cstring_len. *)
+(*       entailer!. *)
+(*       apply repr_inj_unsigned; *)
+(*         first [ apply get_keyslice_inrange | assumption ]. *)
+(*     } *)
+(*     forward_if (temp _t'12 (if Trie.create_pair_aux_dec k1 k2 then Vint Int.one else Vint Int.zero)). *)
+(*     { *)
+(*       forward. *)
+(*       entailer!. *)
+(*       if_tac. *)
+(*       - reflexivity. *)
+(*       - rep_omega. *)
+(*     } *)
+(*     { *)
+(*       forward. *)
+(*       entailer!. *)
+(*       if_tac. *)
+(*       + assert (Zlength k2 <= keyslice_length) by rep_omega. *)
+(*         destruct (Int.ltu (Int.repr 4) (Int.repr (Zlength k2))) eqn:Heqn. *)
+(*         * apply ltu_inv in Heqn. *)
+(*           rewrite ?Int.unsigned_repr in Heqn by rep_omega. *)
+(*           rep_omega. *)
+(*         * reflexivity. *)
+(*       + destruct (Int.ltu (Int.repr 4) (Int.repr (Zlength k2))) eqn:Heqn. *)
+(*         * reflexivity. *)
+(*         * apply ltu_false_inv in Heqn. *)
+(*           rewrite ?Int.unsigned_repr in Heqn by rep_omega. *)
+(*           rep_omega. *)
+(*     } *)
+(*     forward_if. *)
+(*     + if_tac in H7; try solve [inv H7]. *)
+(*       forward_call tt. *)
+(*       Intros pbnode. *)
+(*       forward_call (k1, pk1). *)
+(*       Intros pk1'. *)
+(*       forward_call (Tsh, k1, pk1', Tsh, @BorderNode.empty val _, pbnode, v1). *)
+(*       forward_call (k2, pk2). *)
+(*       Intros pk2'. *)
+(*       forward_call (Tsh, k2, pk2', Tsh, (BorderNode.put_value k1 v1 BorderNode.empty), pbnode, v2). *)
+(*       forward_call (k1, pk1'). *)
+(*       forward_call (k2, pk2'). *)
+(*       forward_call tt. *)
+(*       Intros vret. *)
+(*       destruct vret as [t pt]. *)
+(*       simpl fst in *. *)
+(*       simpl snd in *. *)
+(*       pose proof (BTree.empty_correct _ H9). *)
+(*       forward_call (t, pt). *)
+(*       Intros pc. *)
+(*       forward_call ((get_keyslice k1), pbnode, t, pt, (BTree.first_cursor t), pc). *)
+(*       { apply BTree.first_cursor_abs; assumption. } *)
+(*       Intros vret. *)
+(*       destruct vret as [tableform tablecursor]. *)
+(*       simpl fst in *. *)
+(*       simpl snd in *. *)
+(*       forward_call (tablecursor, pc). *)
+(*       forward. *)
+(*       pose (bnode := BorderNode.put_value k2 (Trie.value_of v2) *)
+(*                                           (BorderNode.put_value k1 (Trie.value_of v1) BorderNode.empty)). *)
+(*       pose (listform := BTree.Flattened.put_aux (get_keyslice k1) (pbnode, bnode) []). *)
+(*       Exists (Trie.trienode_of pt tableform listform). *)
+(*       Exists pt. *)
+(*       Exists [(Trie.trienode_of pt tableform listform, tablecursor, bnode, BorderNode.length_to_cursor (Zlength k1))]. *)
+(*       entailer!. *)
+(*       * eapply Trie.create_pair_case1 with (listform0 := listform); *)
+(*           unfold BTree.Flattened.put, BTree.Flattened.empty, listform; *)
+(*           repeat match goal with *)
+(*                  | [|- _ /\ _] => *)
+(*                    split *)
+(*                  end; *)
+(*           eauto. *)
+(*       * unfold listform. *)
+(*         simpl. *)
+(*         entailer!. *)
+(*         -- unfold Trie.key_inrange. *)
+(*            repeat first [ apply get_keyslice_inrange | constructor ]. *)
+(*         -- unfold bnode, BorderNode.put_value. *)
+(*            simpl. *)
+(*            if_tac; if_tac; *)
+(*              simpl; *)
+(*              rewrite ?Forall_map; *)
+(*              rewrite <- ?upd_Znth_map; *)
+(*              rewrite ?map_list_repeat; *)
+(*              simpl; *)
+(*              entailer!; *)
+(*              repeat match goal with *)
+(*                     | |- _ /\ _ => split *)
+(*                     | |- Forall _ (upd_Znth _ _ _) => *)
+(*                       apply Forall_upd_Znth; [list_solve | | ] *)
+(*                     | |- Forall _ (list_repeat _ _) => *)
+(*                       apply Forall_list_repeat *)
+(*                     | _ => solve [auto] *)
+(*                     end. *)
+(*     + if_tac in H7; try solve [inv H7]. *)
+(*       forward_call tt. *)
+(*       Intros pbnode. *)
+(*       rewrite (cstring_len_split _ k1 pk1 keyslice_length) by rep_omega. *)
+(*       rewrite (cstring_len_split _ k2 pk2 keyslice_length) by rep_omega. *)
+(*       Intros. *)
+(*       forward_call ((sublist keyslice_length (Zlength k1) k1), *)
+(*                     (sublist keyslice_length (Zlength k2) k2), *)
+(*                     (field_address (tarray tschar (Zlength k1)) [ArraySubsc keyslice_length] pk1), *)
+(*                     (field_address (tarray tschar (Zlength k2)) [ArraySubsc keyslice_length] pk2), *)
+(*                     v1, v2). *)
+(*       { *)
+(*         entailer!. *)
+(*         rewrite ?field_address_offset by (auto with field_compatible). *)
+(*         rewrite ?Zlength_sublist by rep_omega. *)
+(*         repeat constructor. *)
+(*       } *)
+(*       { *)
+(*         rewrite ?Zlength_sublist by rep_omega. *)
+(*         repeat first [ split | rep_omega | auto ]. *)
+(*       } *)
+(*       Intros vret. *)
+(*       destruct vret as [[t' pt'] c']. *)
+(*       simpl fst in *. *)
+(*       simpl snd in *. *)
+(*       forward_call (Tsh, @BorderNode.empty val _, pbnode, pt'). *)
+(*       forward_call tt. *)
+(*       Intros vret. *)
+(*       destruct vret as [t pt]. *)
+(*       simpl fst in *. *)
+(*       simpl snd in *. *)
+(*       pose proof (BTree.empty_correct _ H12). *)
+(*       forward_call (t, pt). *)
+(*       Intros pc. *)
+(*       forward_call ((get_keyslice k1), pbnode, t, pt, (BTree.first_cursor t), pc). *)
+(*       { apply BTree.first_cursor_abs; assumption. } *)
+(*       Intros vret. *)
+(*       destruct vret as [tableform tablecursor]. *)
+(*       simpl fst in *. *)
+(*       simpl snd in *. *)
+(*       forward_call (tablecursor, pc). *)
+(*       forward. *)
+(*       pose (bnode := BorderNode.put_suffix None (Trie.trie_of t') BorderNode.empty). *)
+(*       pose (listform := BTree.Flattened.put_aux (get_keyslice k1) (pbnode, bnode) []). *)
+(*       Exists (Trie.trienode_of pt tableform listform). *)
+(*       Exists pt. *)
+(*       Exists ((Trie.trienode_of pt tableform listform, tablecursor, bnode, BorderNode.before_suffix) :: c'). *)
+(*       entailer!. *)
+(*       * eapply Trie.create_pair_case2 with (listform0 := listform); *)
+(*           unfold BTree.Flattened.put, BTree.Flattened.empty, listform; *)
+(*           repeat match goal with *)
+(*                  | [|- _ /\ _] => *)
+(*                    split *)
+(*                  end; *)
+(*           eauto; rep_omega. *)
+(*       * unfold listform. *)
+(*         simpl. *)
+(*         entailer!. *)
+(*         -- unfold Trie.key_inrange. *)
+(*            repeat first [ apply get_keyslice_inrange | constructor ]. *)
+(*         -- unfold bnode, BorderNode.put_value. *)
+(*            simpl. *)
+(*            Exists pt'. *)
+(*            rewrite (cstring_len_split _ k1 pk1 keyslice_length) by rep_omega. *)
+(*            rewrite (cstring_len_split _ k2 pk2 keyslice_length) by rep_omega. *)
+(*            entailer!. *)
+(*   - forward_call tt. *)
+(*     Intros pbnode1. *)
+(*     forward_call (k1, pk1). *)
+(*     Intros pk1'. *)
+(*     forward_call (Tsh, k1, pk1', Tsh, @BorderNode.empty val _, pbnode1, v1). *)
+(*     forward_call tt. *)
+(*     Intros pbnode2. *)
+(*     forward_call (k2, pk2). *)
+(*     Intros pk2'. *)
+(*     forward_call (Tsh, k2, pk2', Tsh, @BorderNode.empty val _, pbnode2, v2). *)
+(*     forward_call (k1, pk1'). *)
+(*     forward_call (k2, pk2'). *)
+(*     forward_call tt. *)
+(*     Intros vret. *)
+(*     destruct vret as [t pt]. *)
+(*     simpl fst in *. *)
+(*     simpl snd in *. *)
+(*     pose proof (BTree.empty_correct _ H4). *)
+(*     forward_call (t, pt). *)
+(*     Intros pc2. *)
+(*     forward_call ((get_keyslice k2), pbnode2, t, pt, (BTree.first_cursor t), pc2). *)
+(*     { apply BTree.first_cursor_abs; assumption. } *)
+(*     Intros vret. *)
+(*     destruct vret as [tableform2 tablecursor2]. *)
+(*     simpl fst in *. *)
+(*     simpl snd in *. *)
+(*     forward_call (tablecursor2, pc2). *)
+(*     pose proof H6. *)
+(*     apply BTree.put_correct in H6; [ | apply BTree.first_cursor_abs; assumption ]. *)
+(*     forward_call (tableform2, pt). *)
+(*     Intros pc1. *)
+(*     forward_call ((get_keyslice k1), pbnode1, tableform2, pt, (BTree.first_cursor tableform2), pc1). *)
+(*     { apply BTree.first_cursor_abs; assumption. } *)
+(*     Intros vret. *)
+(*     destruct vret as [tableform1 tablecursor1]. *)
+(*     simpl fst in *. *)
+(*     simpl snd in *. *)
+(*     forward_call (tablecursor1, pc1). *)
+(*     forward. *)
+(*     pose (bnode1 := BorderNode.put_value k1 (Trie.value_of v1) BorderNode.empty). *)
+(*     pose (bnode2 := BorderNode.put_value k2 (Trie.value_of v2) BorderNode.empty). *)
+(*     pose (listform2 := BTree.Flattened.put_aux (get_keyslice k2) (pbnode2, bnode2) []). *)
+(*     pose (listform1 := BTree.Flattened.put_aux (get_keyslice k1) (pbnode1, bnode1) listform2). *)
+(*     Exists (Trie.trienode_of pt tableform1 listform1). *)
+(*     Exists pt. *)
+(*     Exists [(Trie.trienode_of pt tableform1 listform1, tablecursor1, bnode1, BorderNode.length_to_cursor (Zlength k1))]. *)
+(*     assert (get_keyslice k1 <> get_keyslice k2). { *)
+(*       intro. *)
+(*       apply H3. *)
+(*       f_equal. *)
+(*       assumption. *)
+(*     } *)
+(*     entailer!. *)
+(*     + eapply Trie.create_pair_case3 with (listform3 := listform1) (listform4 := listform2); *)
+(*         unfold BTree.Flattened.put, BTree.Flattened.empty, listform1, listform2; *)
+(*         repeat match goal with *)
+(*         | [|- _ /\ _] => *)
+(*           split *)
+(*         end; *)
+(*         eauto. *)
+(*     + unfold listform1, listform2. *)
+(*       simpl. *)
+(*       if_tac. *)
+(*       * entailer!. *)
+(*         -- unfold Trie.key_inrange. *)
+(*            repeat first [ apply get_keyslice_inrange | constructor ]. *)
+(*         -- unfold iter_sepcon. *)
+(*            unfold bnode1, bnode2, BorderNode.put_value. *)
+(*            simpl. *)
+(*            repeat if_tac; *)
+(*              rewrite ?Forall_map; *)
+(*              rewrite <- ?upd_Znth_map; *)
+(*              rewrite ?map_list_repeat; *)
+(*              simpl; *)
+(*              entailer!; *)
+(*              repeat match goal with *)
+(*                     | |- _ /\ _ => split *)
+(*                     | |- Forall _ (upd_Znth _ _ _) => *)
+(*                       apply Forall_upd_Znth; [list_solve | | ] *)
+(*                     | |- Forall _ (list_repeat _ _) => *)
+(*                       apply Forall_list_repeat *)
+(*                     | _ => solve [auto] *)
+(*                     end. *)
+(*       * entailer!. *)
+(*         rewrite ?if_false by auto. *)
+(*         -- unfold Trie.key_inrange. *)
+(*            repeat first [ apply get_keyslice_inrange | constructor ]. *)
+(*         -- unfold iter_sepcon. *)
+(*            unfold bnode1, bnode2, BorderNode.put_value. *)
+(*            rewrite ?(if_false _ (BTree.Flattened.KeyFacts.eq_dec (get_keyslice k1) (get_keyslice k2))) by auto. *)
+(*            simpl. *)
+(*            repeat if_tac; *)
+(*              rewrite ?Forall_map; *)
+(*              rewrite <- ?upd_Znth_map; *)
+(*              rewrite ?map_list_repeat; *)
+(*              simpl; *)
+(*              entailer!; *)
+(*              repeat match goal with *)
+(*                     | |- _ /\ _ => split *)
+(*                     | |- Forall _ (upd_Znth _ _ _) => *)
+(*                       apply Forall_upd_Znth; [list_solve | | ] *)
+(*                     | |- Forall _ (list_repeat _ _) => *)
+(*                       apply Forall_list_repeat *)
+(*                     | _ => solve [auto] *)
+(*                     end. *)
+(* Qed. *)
